\paragraph{Vis at det finnes en funksjon} \mbox{} \\
$$z = g(x,y)$$
s.a. $g = \text{uttrykk med g(x,y)}$.
\\\\
Skriv om med z istedenfor: $z = \text{uttrykk med z}$.
Flytt rundt s√• uttrykket blir 0 og kall dette $f(x,y)$.
$$\frac{\partial f}{\partial z}(\vec{a}, g(\vec{a})) \neq 0$$

\paragraph{deriverte} \mbox{} \\
$$\frac{\partial g}{\partial x(\vec{a})}
  = -\frac{\frac{\partial f}{\partial x}(\vec{a},g(\vec{a}))}
          {\frac{\partial f}{\partial z}(\vec{a},g(\vec{a}))}$$
og
$$\frac{\partial g}{\partial y(\vec{a})}
  = -\frac{\frac{\partial f}{\partial y}(\vec{a},g(\vec{a}))}
          {\frac{\partial f}{\partial z}(\vec{a},g(\vec{a}))}$$
